src/Lambda/LambdaCalculus.v
@@ -1,14 +1,10 @@
-Require Import List.
+From Stdlib Require Import Bool Arith List.
 Import ListNotations.
-
-Require Import Bool.
 
 Parameter V : Type.
 Parameter dec : V -> V -> bool.
 Parameter dec_spec :
   forall x y : V, reflect (x = y) (dec x y).
-
-Require Import Arith.
 
 Notation "x =? y" := (dec x y) (at level 70).
 
